src/ILEnv.v
@@ -1,0 +1,166 @@
+(** This file contains generic environment information for the Bedrock IL
+ **)
+Require Import List.
+Require Import Word.
+Require Import Expr.
+Require Import Env.
+Require Import Memory IL.
+
+Set Implicit Arguments.
+Set Strict Implicit.
+
+Definition bedrock_types_r : Repr Expr.type :=
+{| footprint := (
+   (0, {| Expr.Impl := W 
+        ; Expr.Eq := fun x y => 
+          match weq x y with
+            | left pf => Some pf 
+            | _ => None 
+          end
+        |}) ::
+   (1, {| Expr.Impl := settings * state
+        ; Expr.Eq := fun _ _ => None
+        |}) ::
+   (2, {| Expr.Impl := state
+        ; Expr.Eq := fun _ _ => None
+        |}) ::
+   (3, {| Expr.Impl := IL.test
+        ; Expr.Eq := fun l r => 
+          match l as l , r as r with
+            | IL.Eq , IL.Eq => Some (refl_equal _)
+            | IL.Ne , IL.Ne => Some (refl_equal _)
+            | IL.Le , IL.Le => Some (refl_equal _)
+            | IL.Lt , IL.Lt => Some (refl_equal _)
+            | _ , _ => None
+          end
+        |}) ::
+   (4, {| Expr.Impl := IL.reg
+        ; Expr.Eq := fun l r =>
+          match l as l , r as r with
+            | IL.Sp , IL.Sp => Some (refl_equal _)
+            | IL.Rp , IL.Rp => Some (refl_equal _)
+            | IL.Rv , IL.Rv => Some (refl_equal _)
+            | _ , _ => None
+          end
+        |}) :: nil) :: nil
+ ; default := Expr.EmptySet_type
+ |}.
+
+Definition bedrock_types : list Expr.type :=
+  Eval cbv beta iota zeta delta 
+    [ repr repr' fold_right default footprint bedrock_types_r updateAt
+      hd hd_error value error tl
+    ]
+    in repr bedrock_types_r nil.
+
+Definition comparator (t : IL.test) (l r : W) : Prop :=
+  match t with
+    | IL.Eq => l = r
+    | IL.Ne => l = r -> False
+    | IL.Lt => wlt l r
+    | IL.Le => wlt l r \/ l = r
+  end.
+
+Section typed_ext.
+  Variable types' : list type.
+  Local Notation "'TYPES'" := (repr bedrock_types_r types').
+
+  Local Notation "'pcT'" := (tvType 0).
+  Local Notation "'tvWord'" := (tvType 0).
+  Local Notation "'stT'" := (tvType 1).
+  Local Notation "'tvState'" := (tvType 2).
+  Local Notation "'tvTest'" := (tvType 3).
+  Local Notation "'tvReg'" := (tvType 4).
+
+  Definition bedrock_funcs_r : Repr (signature (repr bedrock_types_r types')).
+  refine (
+    {| default := Default_signature _
+      ; footprint := (
+        (0, {| Domain := tvWord :: tvWord :: nil
+          ; Range := tvWord
+          ; Denotation := _ |}) ::
+        (1, {| Domain := tvWord :: tvWord :: nil
+          ; Range := tvWord
+          ; Denotation := _ |}) ::
+        (2, {| Domain := tvWord :: tvWord :: nil
+          ; Range := tvWord
+          ; Denotation := _ |}) ::
+        (3, {| Domain := tvTest :: tvWord :: tvWord :: nil
+          ; Range := tvProp
+          ; Denotation := _ |}) :: 
+        (4, {| Domain := tvState :: tvReg :: nil
+          ; Range := tvWord
+          ; Denotation := _ |}) :: nil) :: nil
+    |});
+  cbv beta iota zeta delta [ functionTypeD map ]; (repeat rewrite tvarD_repr_repr_get); simpl.
+  refine (@wplus 32).
+  refine (@wminus 32).
+  refine (@wmult 32).
+  refine comparator.
+  refine Regs.
+  Defined.
+
+  Definition bedrock_funcs : functions (repr bedrock_types_r types') :=
+    Eval cbv beta iota zeta delta 
+      [ repr repr' default footprint fold_right bedrock_funcs_r updateAt hd_error error value
+        bedrock_types_r Default_signature tl hd ]
+      in repr bedrock_funcs_r nil.
+  
+  Variable funcs' : functions TYPES.
+  Definition funcs := repr bedrock_funcs_r funcs'.
+  
+  Definition fPlus (l r : expr TYPES) : expr TYPES :=
+    Expr.Func 0 (l :: r :: nil).
+  Definition fMinus (l r : expr TYPES) : expr TYPES :=
+    Expr.Func 1 (l :: r :: nil).
+  Definition fMult (l r : expr TYPES) : expr TYPES :=
+    Expr.Func 2 (l :: r :: nil).
+
+  Theorem fPlus_correct : forall l r uvars vars, 
+    match exprD funcs uvars vars l (tvType 0) , exprD funcs uvars vars r (tvType 0) with
+      | Some lv , Some rv =>
+        exprD funcs uvars vars (fPlus l r) (tvType 0) = Some (wplus lv rv)
+      | _ , _ => True
+    end.
+  Proof.
+    intros; simpl; unfold eq_ind_r; simpl;
+      repeat match goal with
+               | [ |- match ?X with
+                        | Some _ => _
+                        | None => _
+                      end ] => destruct X
+             end; auto.
+  Qed.
+  Theorem fMinus_correct : forall l r uvars vars, 
+    match exprD funcs uvars vars l tvWord , exprD funcs uvars vars r tvWord with
+      | Some lv , Some rv =>
+        exprD funcs uvars vars (fMinus l r) tvWord = Some (wminus lv rv)
+      | _ , _ => True
+    end.
+  Proof.
+    intros; simpl; unfold eq_ind_r; simpl;
+      repeat match goal with
+               | [ |- match ?X with
+                        | Some _ => _
+                        | None => _
+                      end ] => destruct X
+             end; auto.
+  Qed.
+  Theorem fMult_correct : forall l r uvars vars, 
+    match exprD funcs uvars vars l tvWord , exprD funcs uvars vars r tvWord with
+      | Some lv , Some rv =>
+        exprD funcs uvars vars (fMult l r) tvWord = Some (wmult lv rv)
+      | _ , _ => True
+    end.
+  Proof.
+    intros; simpl; unfold eq_ind_r; simpl;
+      repeat match goal with
+               | [ |- match ?X with
+                        | Some _ => _
+                        | None => _
+                      end ] => destruct X
+             end; auto.
+  Qed.
+End typed_ext.
+
+
